fix?

src/ThreadsURA.v
@@ -6,36 +6,40 @@ From Fairness Require Import Mod.
 
 Set Implicit Arguments.
 
-Definition _thsRA {A: Type}: URA.t := (thread_id ==> (Excl.t A))%ra.
-Compute (URA.car (t:=_thsRA)).
-Global Instance thsRA {A: Type}: URA.t := Auth.t (@_thsRA A).
+(* Definition _thsRA {A: Type}: URA.t := Auth.t (Excl.t A). *)
+Global Instance thsRA {A: Type}: URA.t := (thread_id ==> Auth.t (Excl.t A))%ra.
+(* Compute (URA.car (t:=_thsRA)). *)
+(* Global Instance thsRA {A: Type}: URA.t := Auth.t (@_thsRA A). *)
 Compute (URA.car).
 
 Section THHAS.
 
-  Definition _th_has {A: Type} (tid: thread_id) (a: A): (@_thsRA A) :=
-    fun _tid => if (tid_dec _tid tid) then (Some a) else ε.
+  Definition ae_white {A} (a: A) := @Auth.white (Excl.t A) (Some a).
+  Definition ae_black {A} (a: A) := @Auth.black (Excl.t A) (Some a).
+
+  Definition th_has {A: Type} (tid: thread_id) (a: A): (@thsRA A) :=
+    fun _tid => if (tid_dec _tid tid) then ae_white a else ε.
 
   Lemma unfold_th_has {A} tid (a: A):
-    _th_has tid a = fun _tid => if (tid_dec _tid tid) then (Some a) else ε.
+    th_has tid a = fun _tid => if (tid_dec _tid tid) then ae_white a else ε.
   Proof. reflexivity. Qed.
 
-  Definition th_has {A: Type} (tid: thread_id) (a: A): @thsRA A := Auth.black (_th_has tid a).
+  (* Definition th_has {A: Type} (tid: thread_id) (a: A): @thsRA A := Auth.black (_th_has tid a). *)
 
   (* properties *)
-  Lemma _th_has_hit {A: Type}: forall tid (a: A), (_th_has tid a) tid = Some a.
-  Proof. i. rewrite unfold_th_has. unfold _th_has. des_ifs. Qed.
+  Lemma th_has_hit {A: Type}: forall tid (a: A), (th_has tid a) tid = ae_white a.
+  Proof. i. rewrite unfold_th_has. des_ifs. Qed.
 
-  Lemma _th_has_miss {A: Type}: forall tid tid' (MISS: tid <> tid') (a: A), (_th_has tid a tid') = ε.
+  Lemma _th_has_miss {A: Type}: forall tid tid' (MISS: tid <> tid') (a: A), (th_has tid a tid') = ε.
   Proof. i. rewrite unfold_th_has. des_ifs. Qed.
 
   Lemma _th_has_disj {A: Type}: forall tid0 tid1 (a0 a1: A),
-      URA.wf (_th_has tid0 a0 ⋅ _th_has tid1 a1) -> tid0 <> tid1.
-  Proof. ii. do 2 ur in H. clarify. specialize (H tid1). rewrite !_th_has_hit in H. ss. Qed.
+      URA.wf (th_has tid0 a0 ⋅ th_has tid1 a1) -> tid0 <> tid1.
+  Proof. ii. do 2 ur in H. clarify. specialize (H tid1). rewrite !th_has_hit in H. ss. ur in H. ss. Qed.
 
 End THHAS.
 Notation "tid |-> a" := (th_has tid a) (at level 20).
-Global Opaque _th_has.
+Global Opaque th_has.
 
 (* black + delta --> new_black *)
 Definition add_delta_to_black `{M: URA.t} (b: Auth.t M) (w: Auth.t _): Auth.t _ :=
