src/YOrd2Stid.v
@@ -129,25 +129,28 @@ Section PROOF.
 
   Let M2 {R0 R1}: URA.t := URA.prod (@thsRA (prod_WF (wf_stt R0 R1) (wf_stt R0 R1)).(T)) M.
 
-  Definition shared_thsRA_white {R0 R1}
-             (ost: NatMap.t (prod_WF (wf_stt R0 R1) (wf_stt R0 R1)).(T)): @_thsRA (prod_WF (wf_stt R0 R1) (wf_stt R0 R1)).(T) :=
-    fun tid => match NatMap.find tid ost with
-            | Some osot => Some osot
-            | None => Some (wf_stt0 R0 R1, wf_stt0 R0 R1)
-            end.
+  (* Definition shared_thsRA_white {R0 R1} *)
+  (*            (ost: NatMap.t (prod_WF (wf_stt R0 R1) (wf_stt R0 R1)).(T)): @_thsRA (prod_WF (wf_stt R0 R1) (wf_stt R0 R1)).(T) := *)
+  (*   fun tid => match NatMap.find tid ost with *)
+  (*           | Some osot => Some osot *)
+  (*           | None => Some (wf_stt0 R0 R1, wf_stt0 R0 R1) *)
+  (*           end. *)
 
-  Definition shared_thsRA_black {R0 R1}
-             (ost: NatMap.t (prod_WF (wf_stt R0 R1) (wf_stt R0 R1)).(T)): @_thsRA (prod_WF (wf_stt R0 R1) (wf_stt R0 R1)).(T) :=
-    fun tid => match NatMap.find tid ost with
-            | Some osot => ε
-            | None => Some (wf_stt0 R0 R1, wf_stt0 R0 R1)
-            end.
+  (* Definition shared_thsRA_black {R0 R1} *)
+  (*            (ost: NatMap.t (prod_WF (wf_stt R0 R1) (wf_stt R0 R1)).(T)): @_thsRA (prod_WF (wf_stt R0 R1) (wf_stt R0 R1)).(T) := *)
+  (*   fun tid => match NatMap.find tid ost with *)
+  (*           | Some osot => ε *)
+  (*           | None => Some (wf_stt0 R0 R1, wf_stt0 R0 R1) *)
+  (*           end. *)
 
   Definition shared_thsRA {R0 R1}
              (ths_r: (@thsRA (prod_WF (wf_stt R0 R1) (wf_stt R0 R1)).(T)))
              (ost: NatMap.t (prod_WF (wf_stt R0 R1) (wf_stt R0 R1)).(T))
     :=
-    ths_r = (Auth.white (shared_thsRA_white ost)) ⋅ (Auth.black (shared_thsRA_black ost)).
+    ths_r = (fun tid => match NatMap.find tid ost with
+                     | Some osot => ae_black osot
+                     | None => ae_black (wf_stt0 R0 R1, wf_stt0 R0 R1) ⋅ ae_white (wf_stt0 R0 R1, wf_stt0 R0 R1)
+                     end).
 
   Definition I2 {R0 R1}: (@shared2 R0 R1) -> (@URA.car (@M2 R0 R1)) -> Prop :=
     fun '(ths, im_src, im_tgt, st_src, st_tgt) '(ths_r, r) =>
@@ -155,7 +158,7 @@ Section PROOF.
         (<<MK: exists (ost: NatMap.t (prod_WF (wf_stt R0 R1) (wf_stt R0 R1)).(T)),
             (<<WFOST: nm_wf_pair ths ost>>) /\
               (<<TRES: shared_thsRA ths_r ost>>) /\
-              (<<IMSRC: forall tid (IN: NatMap.In tid ost)
+              (<<IMSRC: forall tid (IN: NatMap.In tid ths)
                           os ot (FIND: NatMap.find tid ost = Some (os, ot)),
                   wf_src_th.(lt) ((ot, im_tgt (inl tid)), nm_proj_v1 ost) ((imap_proj_wf1 im_src) (inl tid))>>)
                 >>).
